Sketch of morello specilization

model/coq/Morello.v
@@ -2,8 +2,10 @@
 
 Require Import Cheri.Capabilities.
 Require Import StructTact.StructTactics.
+Require Import Coq.Vectors.VectorDef.
 
 Require Import bbv.Word.
+Import VectorNotations.
 Import bbv.Word.Notations.
 
 Local Open Scope word_scope.
@@ -12,6 +14,8 @@ Definition w64_size: nat := 64.
 Definition w64 := word w64_size.
 Definition w64_lt: w64 -> w64 -> Prop := @wlt w64_size.
 Definition w64_interval : Type := Interval w64_lt.
+
+Definition w8 := word 8.
 
 Lemma w64_lt_irref: forall x:w64, ~ w64_lt x x.
 Proof.
@@ -43,6 +47,7 @@ Definition otype := word otype_size.
 
 Record MPermission :=
   {
+  global: bool;
   permits_load: bool;
   permits_store: bool;
   permits_execute: bool ;
@@ -64,6 +69,8 @@ Record MPermission :=
 
 Instance CPermissoin_MPermission: CPermission(MPermission) :=
   {|
+  Capabilities.global :=
+    fun p : MPermission => global p = true;
   Capabilities.permits_execute :=
     fun p : MPermission => permits_execute p = true;
   Capabilities.permits_ccall :=
@@ -124,9 +131,9 @@ Record MCapability :=
   value_addr: w64;
   value_otype: MObjectType;
 
-  bounds: w64_interval; (* TODO: alignment *)
+  bounds: w64_interval;
+  flags: w8;
   perms: MPermission;
-  is_global: bool;
   is_execuvite : bool; (* Morello-spefic? *)
 
   obj_type : otype;
@@ -134,7 +141,7 @@ Record MCapability :=
 
 (* @thomas "In the Morello proof we treat RB as sentry and {LPB,LB} as indirect sentries."
    TODO: probably we can do this more elegantly w/o using Program.
-*)
+ *)
 Program Definition Seal_of_otype (x:otype): (@CapSeal MObjectType)
   :=
     if weq x CAP_SEAL_TYPE_UNSEALED then Cap_Unsealed
@@ -162,53 +169,39 @@ Program Definition otype_of_w64 (ot:w64): option MObjectType
 Program Definition address_of_otype (ot:MObjectType): w64
   := zext (proj1_sig ot) (w64_size-otype_size).
 
-Definition clear_global (c:MCapability): MCapability :=
+Definition munseal (c k:MCapability): MCapability :=
   {|
   is_valid := is_valid c;
   value_addr := value_addr c;
   value_otype := value_otype c;
   bounds := bounds c;
   perms := perms c;
-  is_global := false ;
-  is_execuvite := is_execuvite c;
-  obj_type := obj_type c
-  |}.
-
-Definition unseal (c:MCapability): MCapability :=
-  {|
-  is_valid := is_valid c;
-  value_addr := value_addr c;
-  value_otype := value_otype c;
-  bounds := bounds c;
-  perms := perms c;
-  is_global := is_global c;
+  flags := flags c;
   is_execuvite := is_execuvite c;
   obj_type := CAP_SEAL_TYPE_UNSEALED
   |}.
 
-Definition seal (c:MCapability) (ot:MObjectType): MCapability :=
-  {|
-  is_valid := is_valid c;
-  value_addr := value_addr c;
-  value_otype := value_otype c;
-  bounds := bounds c;
-  perms := perms c;
-  is_global := is_global c;
-  is_execuvite := is_execuvite c;
-  obj_type := proj1_sig ot
-  |}.
-
-Program Definition get_value (c:MCapability) : @CapValue MObjectType w64 :=
+Program Definition mget_value (c:MCapability) : @CapValue MObjectType w64 :=
   if orb (permits_seal (perms c)) (permits_unseal (perms c))
   then CapToken (value_otype c)
   else CapAddress (value_addr c).
 
+(* TODO *)
+Definition mset_value (c:MCapability) (v:@CapValue MObjectType w64): MCapability :=
+  match v with
+  | CapToken t => c
+  | CapAddress a => c
+  end.
+
+Definition mseal (c k:MCapability): MCapability :=
+  mset_value c (mget_value k).
+
 Lemma seal_perms_value_type (c: MCapability):
   permits_seal (perms c) = true \/ permits_unseal (perms c) = true
   <->
-  (exists t : MObjectType, get_value  c = CapToken t).
+  (exists t : MObjectType, mget_value  c = CapToken t).
 Proof.
-  split; unfold get_value; intros.
+  split; unfold mget_value; intros.
   -
     rewrite <- Bool.orb_true_iff in H.
     rewrite H.
@@ -223,31 +216,74 @@ Proof.
       inversion H.
 Qed.
 
+Definition w2v {n:nat}: word n -> vector bool n.
+Admitted.
+
+Parameter M0:MCapability. (* TODO *)
+
+Definition maddr_representable: w64_interval -> w64 -> Prop.
+Admitted.
+
+Definition mbounds_representable_exactly: w64_interval -> Prop.
+Admitted.
+
+
 Instance CCapability_MCapability :
-  @CCapability MObjectType w64 CAddress_w64 MPermission _ (MCapability) :=
+  @CCapability MObjectType w64 CAddress_w64 MPermission CPermissoin_MPermission MCapability :=
   {|
-  Capabilities.is_valid := fun c => is_valid c = true ;
+  Capabilities.C0 := M0 ;
+  Capabilities.CAP_FLAGS_LEN := 8 ;
   Capabilities.get_bounds := fun c => bounds c ;
   Capabilities.get_perms := fun c => perms c ;
-  Capabilities.get_value := fun c => get_value c;
+  Capabilities.get_value := fun c => mget_value c;
+  Capabilities.get_flags := fun c => w2v (flags c) ;
   Capabilities.get_seal := fun c => Seal_of_otype (obj_type c) ;
-  Capabilities.is_global := fun c => is_global c = true ;
   Capabilities.address_of_otype := address_of_otype ;
   Capabilities.seal_perms_value_type := seal_perms_value_type;
+  Capabilities.addr_representable := maddr_representable;
+  Capabilities.bounds_representable_exactly := mbounds_representable_exactly;
   |}.
 
-Program Instance CCapabilityOps_MCapability :
+
+Definition mnarrow_bounds: MCapability -> w64_interval -> MCapability.
+Admitted.
+
+Definition mnarrow_bounds_exact: MCapability -> w64_interval -> MCapability.
+Admitted.
+
+Definition mnarrow_perms : MCapability -> MPermission -> MCapability.
+Admitted.
+
+Definition mseal_entry: MCapability -> MCapability.
+Admitted.
+
+Definition mseal_indirect_entry: MCapability -> MCapability.
+Admitted.
+
+Definition mseal_indirect_entry_pair: MCapability -> MCapability.
+Admitted.
+
+Definition mset_flags: MCapability -> vector bool CAP_FLAGS_LEN -> MCapability.
+Admitted.
+
+Instance CCapabilityOps_MCapability :
   @CCapabilityOps _ _ _ _ _ _ CCapability_MCapability :=
   {|
-  Capabilities.seal := seal ;
-  Capabilities.unseal := unseal ;
-  Capabilities.clear_global := clear_global;
+  Capabilities.seal := mseal ;
+  Capabilities.unseal := munseal ;
+  Capabilities.set_value := mset_value;
+  Capabilities.narrow_bounds := mnarrow_bounds;
+  Capabilities.narrow_bounds_exact := mnarrow_bounds_exact;
+  Capabilities.narrow_perms := mnarrow_perms;
+  Capabilities.seal_entry := mseal_entry ;
+  Capabilities.seal_indirect_entry := mseal_indirect_entry ;
+  Capabilities.seal_indirect_entry_pair := mseal_indirect_entry_pair ;
+  Capabilities.set_flags := mset_flags ;
   |}.
-
 
 (* --- Decoding/Encoding --- *)
 
 Definition encode: MCapability -> option (word 128).
-  (* TODO *) Admitted.
+(* TODO *) Admitted.
 Definition decode: word 128 -> option MCapability.
-  (* TODO *) Admitted.
+(* TODO *) Admitted.
